Update Memcpy with Bryan's comments

src/arch/x64/interop/Memcpy.fst
@@ -28,7 +28,7 @@ module BS = X64.Bytes_Semantics_s
 open Vale_memcpy
 
 #set-options "--initial_fuel 5 --max_fuel 5 --initial_ifuel 2 --max_ifuel 2"
-let create_initial_state w dst src stack_b (h0:HS.mem{pre_cond h0 dst src /\ B.length stack_b == 24 /\ live h0 stack_b /\ buf_disjoint_from stack_b [dst;src]}) : GTot TS.traceState =
+let create_initial_state is_win dst src stack_b (h0:HS.mem{pre_cond h0 dst src /\ B.length stack_b == 24 /\ live h0 stack_b /\ buf_disjoint_from stack_b [dst;src]}) : GTot TS.traceState =
   let taint_func (x:b8) : GTot taint =
     if StrongExcludedMiddle.strong_excluded_middle (x == dst) then Secret else
     if StrongExcludedMiddle.strong_excluded_middle (x == src) then Secret else
@@ -38,7 +38,7 @@ let create_initial_state w dst src stack_b (h0:HS.mem{pre_cond h0 dst src /\ B.l
   let addr_dst = addrs dst in
   let addr_src = addrs src in
   let addr_stack:nat64 = addrs stack_b + 0 in
-  let regs = if w then (
+  let regs = if is_win then (
     fun r -> begin match r with
       | Rsp -> addr_stack
       | Rcx -> addr_dst
@@ -52,11 +52,11 @@ let create_initial_state w dst src stack_b (h0:HS.mem{pre_cond h0 dst src /\ B.l
       | _ -> init_regs r end)
   in
   let xmms = init_xmms in
-  let (s_b:BS.state) = {BS.ok = true; BS.regs = regs; BS.xmms = xmms; BS.flags = 0; BS.mem = Interop.down_mem mem.hs mem.addrs mem.ptrs} in
+  let (s_b:BS.state) = {BS.ok = true; BS.regs = regs; BS.xmms = xmms; BS.flags = 0; BS.mem = Interop.down_mem h0 addrs buffers} in
   let s0:X64.Memory_i_s.state = {ME.state = s_b; ME.mem = mem} in
   {TS.state = s0; TS.trace = []; TS.memTaint = create_valid_memtaint mem buffers taint_func}
 
-let create_initial_vale_state w dst src stack_b (h0:HS.mem{pre_cond h0 dst src /\ B.length stack_b == 24 /\ live h0 stack_b /\ buf_disjoint_from stack_b [dst;src]}) : GTot va_state =
+let create_initial_vale_state is_win dst src stack_b (h0:HS.mem{pre_cond h0 dst src /\ B.length stack_b == 24 /\ live h0 stack_b /\ buf_disjoint_from stack_b [dst;src]}) : GTot va_state =
   let taint_func (x:b8) : GTot taint =
     if StrongExcludedMiddle.strong_excluded_middle (x == dst) then Secret else
     if StrongExcludedMiddle.strong_excluded_middle (x == src) then Secret else
@@ -66,7 +66,7 @@ let create_initial_vale_state w dst src stack_b (h0:HS.mem{pre_cond h0 dst src /
   let addr_dst = addrs dst in
   let addr_src = addrs src in
   let addr_stack:nat64 = addrs stack_b + 0 in
-  let regs = if w then (
+  let regs = if is_win then (
     fun r -> begin match r with
       | Rsp -> addr_stack
       | Rcx -> addr_dst
@@ -82,11 +82,11 @@ let create_initial_vale_state w dst src stack_b (h0:HS.mem{pre_cond h0 dst src /
   let xmms = init_xmms in
   {ok = true; regs = regs; xmms = xmms; flags = 0; mem = mem; memTaint =    create_valid_memtaint mem buffers taint_func}
 
-let create_lemma w dst src stack_b (h0:HS.mem{pre_cond h0 dst src /\ B.length stack_b == 24 /\ live h0 stack_b /\ buf_disjoint_from stack_b [dst;src]}) : Lemma
-  (state_of_S (create_initial_state w dst src stack_b h0) == create_initial_vale_state w dst src stack_b h0) =
-    let s_init = create_initial_state w dst src stack_b h0 in
+let create_lemma is_win dst src stack_b (h0:HS.mem{pre_cond h0 dst src /\ B.length stack_b == 24 /\ live h0 stack_b /\ buf_disjoint_from stack_b [dst;src]}) : Lemma
+  (state_of_S (create_initial_state is_win dst src stack_b h0) == create_initial_vale_state is_win dst src stack_b h0) =
+    let s_init = create_initial_state is_win dst src stack_b h0 in
     let s0 = state_of_S s_init in
-    let s1 = create_initial_vale_state w dst src stack_b h0 in
+    let s1 = create_initial_vale_state is_win dst src stack_b h0 in
     assert (FunctionalExtensionality.feq s1.regs (regs' s_init.TS.state));
     assert (FunctionalExtensionality.feq s1.xmms (xmms' s_init.TS.state));
     lemma_of_ok s_init;
@@ -97,28 +97,28 @@ let create_lemma w dst src stack_b (h0:HS.mem{pre_cond h0 dst src /\ B.length st
     lemma_of_memTaint s_init;
     ()
 
-let implies_pre (w:bool) (h0:HS.mem) (dst:s8) (src:s8)  (stack_b:b8) : Lemma
+let implies_pre (is_win:bool) (h0:HS.mem) (dst:s8) (src:s8)  (stack_b:b8) : Lemma
   (requires pre_cond h0 dst src /\ B.length stack_b == 24 /\ live h0 stack_b /\ buf_disjoint_from stack_b [dst;src])
   (ensures (
   B.length stack_b == 24 /\ live h0 stack_b /\ buf_disjoint_from stack_b [dst;src] /\ (
-  let s0 = create_initial_vale_state w dst src stack_b h0 in
+  let s0 = create_initial_vale_state is_win dst src stack_b h0 in
   length_t_eq (TBase TUInt64) stack_b;
   length_t_eq (TBase TUInt64) dst;
   length_t_eq (TBase TUInt64) src;
-  va_pre (va_code_memcpy w) s0 w stack_b dst src ))) =
+  va_pre (va_code_memcpy is_win) s0 is_win stack_b dst src ))) =
   length_t_eq (TBase TUInt64) stack_b;
   length_t_eq (TBase TUInt64) dst;
   length_t_eq (TBase TUInt64) src;
-  assert(B.disjoint stack_b dst);
-  assert(B.disjoint stack_b src);
+  assert(Interop.disjoint stack_b dst);
+  assert(Interop.disjoint stack_b src);
   ()
 
 let seq_nat64_to_seq_U64 (b:Seq.seq nat64) : (Seq.seq UInt64.t) =
   Seq.init (Seq.length b) (fun (i:nat { i < Seq.length b }) -> UInt64.uint_to_t (Seq.index b i))
 
-let implies_post (w:bool) (va_s0:va_state) (va_sM:va_state) (va_fM:va_fuel) (dst:s8) (src:s8)  (stack_b:b8) : Lemma
+let implies_post (is_win:bool) (va_s0:va_state) (va_sM:va_state) (va_fM:va_fuel) (dst:s8) (src:s8)  (stack_b:b8) : Lemma
   (requires pre_cond va_s0.mem.hs dst src /\ B.length stack_b == 24 /\ live va_s0.mem.hs stack_b /\ buf_disjoint_from stack_b [dst;src] /\
-    va_post (va_code_memcpy w) va_s0 va_sM va_fM w stack_b dst src )
+    va_post (va_code_memcpy is_win) va_s0 va_sM va_fM is_win stack_b dst src )
   (ensures post_cond va_s0.mem.hs va_sM.mem.hs dst src ) =
   length_t_eq (TBase TUInt64) stack_b;
   length_t_eq (TBase TUInt64) dst;
@@ -130,29 +130,29 @@ let implies_post (w:bool) (va_s0:va_state) (va_sM:va_state) (va_fM:va_fuel) (dst
   assert (Seq.equal (seq_nat64_to_seq_U64 (buffer_as_seq #t (va_get_mem va_sM) dst)) (BV.as_seq va_sM.mem.hs dst_b));  
   ()
 
-val lemma_ghost_memcpy:  w:bool -> dst:s8 -> src:s8 ->  stack_b:b8 -> (h0:HS.mem{pre_cond h0 dst src /\ B.length stack_b == 24 /\ live h0 stack_b /\ buf_disjoint_from stack_b [dst;src]}) ->
+val lemma_ghost_memcpy:  is_win:bool -> dst:s8 -> src:s8 ->  stack_b:b8 -> (h0:HS.mem{pre_cond h0 dst src /\ B.length stack_b == 24 /\ live h0 stack_b /\ buf_disjoint_from stack_b [dst;src]}) ->
   Ghost (TS.traceState * nat * HS.mem)
     (requires True)
     (ensures (fun (s1, f1, h1) ->
-      (let s0 = create_initial_state w dst src stack_b h0 in
-       Some s1 == TS.taint_eval_code (va_code_memcpy w) f1 s0 /\
-       s1.TS.state.ME.state.BS.mem == Interop.down_mem h1 addrs [stack_b;dst;src] /\
+      (let s0 = create_initial_state is_win dst src stack_b h0 in
+       Some s1 == TS.taint_eval_code (va_code_memcpy is_win) f1 s0 /\
+       Interop.correct_down h1 addrs [stack_b;dst;src] s1.TS.state.ME.state.BS.mem /\
        post_cond h0 h1 dst src /\
-       calling_conventions w s0 s1)
+       calling_conventions is_win s0 s1)
       )
     )
 
 
-let lemma_ghost_memcpy w dst src stack_b h0 =
+let lemma_ghost_memcpy is_win dst src stack_b h0 =
   length_t_eq (TBase TUInt64) stack_b;
   length_t_eq (TBase TUInt64) dst;
   length_t_eq (TBase TUInt64) src;
-  implies_pre w h0 dst src stack_b ;
-  let s0 = create_initial_state w dst src stack_b h0 in
-  create_lemma w dst src stack_b h0;
-  let s_v, f_v = va_lemma_memcpy (va_code_memcpy w) (state_of_S s0) w stack_b dst src in  
-  implies_post w (state_of_S s0) s_v f_v dst src stack_b;
-  Some?.v (TS.taint_eval_code (va_code_memcpy w) f_v s0), f_v, s_v.mem.hs
+  implies_pre is_win h0 dst src stack_b ;
+  let s0 = create_initial_state is_win dst src stack_b h0 in
+  create_lemma is_win dst src stack_b h0;
+  let s_v, f_v = va_lemma_memcpy (va_code_memcpy is_win) (state_of_S s0) is_win stack_b dst src in  
+  implies_post is_win (state_of_S s0) s_v f_v dst src stack_b;
+  Some?.v (TS.taint_eval_code (va_code_memcpy is_win) f_v s0), f_v, s_v.mem.hs
 
 let memcpy dst src  =
   push_frame();
